formal/inference/heuristics/Instance_Of.thy
@@ -1,0 +1,7 @@
+theory Instance_Of
+  imports "../Inference"
+begin
+
+  
+
+end
